Wholly remove fborrow

nola/examples/logic/adequacy.v
@@ -11,7 +11,6 @@ Class nintpGpreS Σ := NintpGpreS {
   nintpGpreS_na_inv :: na_invG Σ;
   nintpGpreS_cinv :: cinvG Σ;
   nintpGpreS_borrow :: borrowGpreS (nPropS (;ᵞ)) Σ;
-  nintpGpreS_fborrow :: fborrowGpreS (nPropS (;ᵞ)) Σ;
   nintpGpreS_proph :: prophGpreS nsynty Σ;
   nintpGpreS_proph_ag :: proph_agG nsynty Σ;
   nintpGpreS_heap :: heapGpreS Σ;
@@ -20,14 +19,14 @@ Class nintpGpreS Σ := NintpGpreS {
 (** [gFunctors] for [nintpGpreS] *)
 Definition nintpΣ : gFunctors :=
   #[agreeΣ (nPropL (;ᵞ)); ninvΣ (nPropS (;ᵞ)); na_ninvΣ (nPropS (;ᵞ));
-    na_invΣ; cinvΣ; borrowΣ (nPropS (;ᵞ)); fborrowΣ (nPropS (;ᵞ));
-    prophΣ nsynty; proph_agΣ nsynty; heapΣ].
+    na_invΣ; cinvΣ; borrowΣ (nPropS (;ᵞ)); prophΣ nsynty; proph_agΣ nsynty;
+    heapΣ].
 #[export] Instance subG_nintpGpreS `{!subG nintpΣ Σ} : nintpGpreS Σ.
 Proof. solve_inG. Qed.
 
 (** Whole world satisfaction *)
 Definition nwsatd `{!nintpGS Σ} : iProp Σ :=
-  inv_wsatd ∗ na_inv_wsatd ∗ borrow_wsatd ∗ fborrow_wsat false ∗ proph_wsat.
+  inv_wsatd ∗ na_inv_wsatd ∗ borrow_wsatd ∗ proph_wsat.
 
 (** Adequacy of [wp] over [inv_wsatd] *)
 Lemma wp_n_adequacy `{!nintpGpreS Σ} {s e σ φ} :
@@ -36,11 +35,10 @@ Lemma wp_n_adequacy `{!nintpGpreS Σ} {s e σ φ} :
 Proof.
   move=> towp. apply (heap_adequacy Σ HasNoLc)=> ?.
   iMod inv_wsat_alloc as (?) "W0". iMod na_inv_wsat_alloc as (?) "W1".
-  iMod borrow_wsat_alloc as (?) "W2". iMod fborrow_wsat_alloc as (?) "W3".
-  iMod proph_wsat_alloc as (?) "W4". iModIntro.
-  iDestruct (towp (NintpGS _ _ _ _ _ _ _ _ _ _)) as "big". iExists nwsatd.
-  iFrame "big". iSplitL "W0"; [done|].
-  iSplitL "W1"; [done|]. iSplitL "W2"; [done|]. by iSplitL "W3".
+  iMod borrow_wsat_alloc as (?) "W2". iMod proph_wsat_alloc as (?) "W3".
+  iModIntro. iDestruct (towp (NintpGS _ _ _ _ _ _ _ _ _)) as "big".
+  iExists nwsatd. iFrame "big". iSplitL "W0"; [done|].
+  iSplitL "W1"; [done|]. by iSplitL "W2".
 Qed.
 
 (** Adequacy of [twp] over [inv_wsatd] *)
@@ -50,9 +48,8 @@ Lemma twp_n_adequacy `{!nintpGpreS Σ} {s e σ φ} :
 Proof.
   move=> totwp. apply (heap_total Σ s _ _ φ)=> ?.
   iMod inv_wsat_alloc as (?) "W0". iMod na_inv_wsat_alloc as (?) "W1".
-  iMod borrow_wsat_alloc as (?) "W2". iMod fborrow_wsat_alloc as (?) "W3".
-  iMod proph_wsat_alloc as (?) "W4". iModIntro.
-  iDestruct (totwp (NintpGS _ _ _ _ _ _ _ _ _ _)) as "big". iExists nwsatd.
-  iFrame "big". iSplitL "W0"; [done|].
-  iSplitL "W1"; [done|]. iSplitL "W2"; [done|]. by iSplitL "W3".
+  iMod borrow_wsat_alloc as (?) "W2". iMod proph_wsat_alloc as (?) "W3".
+  iModIntro. iDestruct (totwp (NintpGS _ _ _ _ _ _ _ _ _)) as "big".
+  iExists nwsatd. iFrame "big". iSplitL "W0"; [done|].
+  iSplitL "W1"; [done|]. by iSplitL "W2".
 Qed.
