nola/examples/logic/prop.v
@@ -75,7 +75,6 @@ Variant ncon0 : Type :=
 | (** Dead lifetime token *) nc_lft_dead (α : lft)
 | (** Eternal lifetime token *) nc_lft_eter (α : lft)
 | (** Persistent lifetime inclusion *) nc_lft_sincl (α β : lft)
-| (** Fractured borrowing world satisfaction *) nc_fborrow_wsat
 | (** Prophecy token *) nc_proph_tok (ξ : aprvarn) (q : Qp)
 | (** Prophecy tokens *) nc_proph_toks (ξl : list aprvarn) (q : Qp)
 | (** Prophecy observation *) nc_proph_obs (φπ : prophn Prop)
@@ -195,7 +194,6 @@ Notation "q .[ α ]" := (n_0 (nc_lft_tok α q)) : nProp_scope.
 Notation "[† α ]" := (n_0 (nc_lft_dead α)) : nProp_scope.
 Notation "[∞ α ]" := (n_0 (nc_lft_eter α)) : nProp_scope.
 Notation "α ⊑□ β" := (n_0 (nc_lft_sincl α β)) : nProp_scope.
-Notation n_fborrow_wsat := (n_0 nc_fborrow_wsat).
 Notation n_proph_wsat := (n_0 nc_proph_wsat).
 Notation "q :[ ξ ]" := (n_0 (nc_proph_tok ξ q)) : nProp_scope.
 Notation "q :∗[ ξ ]" := (n_0 (nc_proph_toks ξ q)) : nProp_scope.
